Continue negshift safety

language_formalisation/substitution/substitution_lemmas.v
@@ -39,7 +39,8 @@ reflexivity. apply IHh. apply c_shift_shift.
 }
 Qed.
 
-Lemma v_shift_shift_alt n m cut (v:val) :
+
+(* Lemma v_shift_shift_alt n m cut (v:val) :
   Sub.v_shift (Sub.v_shift v n cut) m (n+cut) = (Sub.v_shift v (n + m) cut)
 
 with c_shift_shift_alt n m cut (c:comp) :
@@ -78,14 +79,14 @@ reflexivity. apply IHh.
 assert (S(S(n+cut))=n+S(S cut)) by omega. rewrite H. 
 apply c_shift_shift_alt.
 }
-Qed.
+Qed. *)
 
 Lemma v_shift_makes_no_var v j:
-  v_no_var_j (Sub.v_shift v 1 j) j
+  v_no_var (Sub.v_shift v 1 j) j
 with c_shift_makes_no_var c j:
-  c_no_var_j (Sub.c_shift c 1 j) j
+  c_no_var (Sub.c_shift c 1 j) j
 with h_shift_makes_no_var h j:
-  h_no_var_j (Sub.h_shift h 1 j) j.
+  h_no_var (Sub.h_shift h 1 j) j.
 Proof.
 {
 clear v_shift_makes_no_var.
@@ -101,14 +102,15 @@ revert j; induction h; intros j; simpl; auto.
 }
 Qed.
 
+
 Lemma v_no_var_shift (v:val) j cut:
-  v_no_var_j v j -> (cut <= j) -> v_no_var_j (Sub.v_shift v 1 cut) (1+j)
+  v_no_var v j -> (cut <= j) -> v_no_var (Sub.v_shift v 1 cut) (1+j)
 
 with c_no_var_shift (c:comp) j cut:
-  c_no_var_j c j -> (cut <= j) -> c_no_var_j (Sub.c_shift c 1 cut) (1+j)
+  c_no_var c j -> (cut <= j) -> c_no_var (Sub.c_shift c 1 cut) (1+j)
   
 with h_no_var_shift (h:hcases) j cut:
-  h_no_var_j h j -> (cut <= j) -> h_no_var_j (Sub.h_shift h 1 cut) (1+j).
+  h_no_var h j -> (cut <= j) -> h_no_var (Sub.h_shift h 1 cut) (1+j).
 Proof.
 {
 clear v_no_var_shift.
@@ -134,13 +136,13 @@ Qed.
 
 
 Lemma v_no_var_sub (v:val) j v_s :
-  v_no_var_j v_s j -> v_no_var_j (Sub.v_sub v (j, v_s)) j
+  v_no_var v_s j -> v_no_var (Sub.v_sub v (j, v_s)) j
 
 with c_no_var_sub (c:comp) j v_s :
-  v_no_var_j v_s j -> c_no_var_j (Sub.c_sub c (j, v_s)) j
+  v_no_var v_s j -> c_no_var (Sub.c_sub c (j, v_s)) j
 
 with h_no_var_sub (h:hcases) j v_s :
-  v_no_var_j v_s j -> h_no_var_j (Sub.h_sub h (j, v_s)) j.
+  v_no_var v_s j -> h_no_var (Sub.h_sub h (j, v_s)) j.
 Proof.
 {
 clear v_no_var_sub.
@@ -159,7 +161,7 @@ try destruct p; simpl; try constructor; auto;
 try apply IHc || apply IHc1 || apply IHc2;
 try (apply v_no_var_shift; assumption || omega).
 all:
-assert (v_no_var_j (Sub.v_shift v_s 1 0) (1 + j)) by
+assert (v_no_var (Sub.v_shift v_s 1 0) (1 + j)) by
   (apply v_no_var_shift; auto || omega);
 apply (v_no_var_shift _ _ 0) in H; try omega.
 all: rewrite v_shift_shift in H; simpl in H; assumption.
@@ -167,15 +169,23 @@ all: rewrite v_shift_shift in H; simpl in H; assumption.
 clear h_no_var_sub.
 revert j v_s. induction h; intros j v_s v_s_clean; simpl; auto.
 constructor. auto.
-assert (v_no_var_j (Sub.v_shift v_s 1 0) (1+j)).
+assert (v_no_var (Sub.v_shift v_s 1 0) (1+j)).
 { apply v_no_var_shift. auto. omega. }
 apply (v_no_var_shift _ _ 0) in H.
 rewrite (v_shift_shift _ _ _) in H. auto. omega.
 }
 Qed.
 
+
 Lemma h_shift_find_op_None h o i j :
   find_op_case h o = None <-> find_op_case (Sub.h_shift h i j) o = None.
+Proof.
+constructor; intro; induction h; auto; simpl in *;
+destruct (o==o0) eqn:cmp; try discriminate; auto.
+Qed.
+
+Lemma h_negshift_find_op_None h o i j :
+  find_op_case h o = None <-> find_op_case (Sub.h_negshift h i j) o = None.
 Proof.
 constructor; intro; induction h; auto; simpl in *;
 destruct (o==o0) eqn:cmp; try discriminate; auto.
@@ -185,6 +195,16 @@ Lemma h_shift_find_op_Some h o i j x k cop :
   find_op_case h o = Some (x, k, cop) -> 
   find_op_case (Sub.h_shift h i j) o = 
     Some (x, k, (Sub.c_shift cop i (2+j))).
+Proof.
+intro; induction h.
++ simpl in H. discriminate.
++ simpl in *. destruct (o==o0) eqn:cmp. inv H. all: auto.
+Qed.
+
+Lemma h_negshift_find_op_Some h o i j x k cop :
+  find_op_case h o = Some (x, k, cop) -> 
+  find_op_case (Sub.h_negshift h i j) o = 
+    Some (x, k, (Sub.c_negshift cop i (2+j))).
 Proof.
 intro; induction h.
 + simpl in H. discriminate.
@@ -211,19 +231,19 @@ intros cmp. induction v; simpl.
 { 
   clear v_shift_comm_aux c_shift_comm_aux h_shift_comm_aux.
   destruct v as (x, dbi).
-  destruct (i<=?dbi) eqn:cmpi; destruct (j<=?dbi) eqn:cmpj; simpl;
-  destruct (d+i<=?dbi) eqn:cmpid; destruct (j<=?n+dbi) eqn:cmpjn; simpl;
-  destruct (d+i<=?d+dbi) eqn:cmpidd; simpl;
-  apply leb_complete in cmpj || apply leb_complete_conv in cmpj;
-  apply leb_complete in cmpi || apply leb_complete_conv in cmpi;
-  apply leb_complete in cmpjn || apply leb_complete_conv in cmpjn;
-  apply leb_complete in cmpid || apply leb_complete_conv in cmpid;
-  apply leb_complete in cmpidd || apply leb_complete_conv in cmpidd;
-  try omega; simpl.  f_equal. f_equal. omega. f_equal. f_equal. omega.
-  { assert (j<=?dbi=true) by (apply leb_correct in cmpj; assumption).
-    rewrite H. auto. }
-  all: assert (j<=?dbi=false) by (apply leb_correct_conv in cmpj; assumption).
-  all: rewrite H; auto.
+  destruct (i<=?dbi) eqn:cmpi; destruct (j<=?dbi) eqn:cmpj; simpl.
+  + apply leb_complete in cmpi. apply leb_complete in cmpj.
+    assert (j<=?n+dbi=true) by (apply leb_correct; omega).
+    assert (d+i<=?d+dbi=true) by (apply leb_correct; omega).
+    rewrite H, H0. f_equal. f_equal. omega.
+  + apply leb_complete in cmpi. apply leb_complete_conv in cmpj. omega.
+  + apply leb_complete_conv in cmpi. rewrite cmpj. apply leb_complete in cmpj.
+    assert (d+i<=?d+dbi=false) by (apply leb_correct_conv; omega).  
+    rewrite H. reflexivity.
+  + rewrite cmpj. 
+    apply leb_complete_conv in cmpi. apply leb_complete_conv in cmpj.
+    assert (d+i<=?dbi=false) by (apply leb_correct_conv; omega).
+    rewrite H.  reflexivity.
 }
 clear v_shift_comm_aux h_shift_comm_aux.
 all: f_equal; auto.
@@ -233,9 +253,10 @@ all: eapply c_shift_comm_aux; omega.
 intros cmp. induction c; simpl; f_equal; auto; 
 clear v_shift_comm_aux h_shift_comm_aux.
 try eapply c_shift_comm_aux; try omega.
-all: assert (S(d+i)=d+S i) by omega; try rewrite H.
-all: assert (S(d+S i)=d+S(S i)) by omega; try rewrite H0.
-all: eapply c_shift_comm_aux; omega.
+all: assert (S(S(d+i))=d+S(S i)) by omega; try (rewrite H;
+  eapply c_shift_comm_aux; omega).
+all: assert (S(d+i)=d+S i) by omega; try rewrite H0;
+  eapply c_shift_comm_aux; omega.
 }{
 clear v_shift_comm_aux h_shift_comm_aux.
 intros cmp. induction h; simpl.
@@ -272,11 +293,11 @@ revert cut. induction v; intros cut m_le_n; simpl; f_equal.
 all : try reflexivity || apply IHv || apply IHv1 || apply IHv2.
 all : try apply c_negshift_shift || apply h_negshift_shift; assumption.
 }{
-clear c_negshift_shift.
+clear c_negshift_shift h_negshift_shift.
 revert cut. induction c; intros cut m_le_n; try destruct p; simpl; f_equal;
 try apply v_negshift_shift || apply IHc || apply IHc1 || apply IHc2; assumption.
 }{
-clear h_negshift_shift.
+clear h_negshift_shift v_negshift_shift.
 revert cut. induction h; intros cut m_le_n; simpl; f_equal.
 reflexivity. apply IHh. assumption. apply c_negshift_shift. assumption.
 }
@@ -326,10 +347,8 @@ clear v_shift_sub c_shift_sub h_shift_sub.
 destruct v as (x, n). 
 destruct (n=?i) eqn:ni.
 apply Nat.eqb_eq in ni. subst.
-++
-  destruct (i=?j) eqn:eqij.
-  {
-    apply Nat.eqb_eq in eqij. subst.
++ destruct (i=?j) eqn:eqij.
+  - apply Nat.eqb_eq in eqij. subst.
     assert (1+j<=?j=false) by (apply leb_correct_conv; omega).
     simpl in H. rewrite H. simpl.
     assert (j=?j=true) by (apply Nat.eqb_eq; reflexivity).
@@ -337,112 +356,236 @@ apply Nat.eqb_eq in ni. subst.
     rewrite v_negshift_shift. rewrite v_negshift_shift.
     rewrite v_shift_shift. rewrite v_shift_shift. f_equal.
     omega. omega.
-  }
-  assert (1+i<=?i=false) by (apply leb_correct_conv; omega).
-  simpl in H. rewrite H. simpl.
-  assert (j<=?i=true) by (apply leb_correct;omega).
-  rewrite H0. rewrite eqij. simpl. rewrite H0.
-  assert (i<=?i-1=false).
-  { apply leb_correct_conv. apply Nat.eqb_neq in eqij. 
-    apply leb_complete in H0. omega. }
-  rewrite H1. reflexivity.
-++ destruct (n=?j) eqn:nj.
-+ apply Nat.eqb_eq in nj. subst.
-  assert (1+i<=?j=false) by (apply leb_correct_conv; omega).
-  simpl in H. rewrite H.
-  simpl. assert (j=?j=true) by (apply Nat.eqb_eq; omega).
-  rewrite H0. rewrite v_negshift_shift. rewrite v_negshift_shift. simpl.
-  rewrite v_shift_0. rewrite v_shift_0.
-  reflexivity. omega. omega.
-+ destruct (i<=?n) eqn:iln; simpl.
-  - destruct (j<=?n) eqn:jln; simpl.
-    * apply leb_complete in jln. apply leb_complete in iln.
-      assert (i<=?n-1=true).
-      { apply leb_correct. apply Nat.eqb_neq in ni. omega. }
-      rewrite H. simpl. assert (1+i<=?n=true).
-      { apply leb_correct. apply leb_complete in H.
-        apply Nat.eqb_neq in ni. omega. }
-      simpl in H0. rewrite H0. simpl. 
-      assert (1+n=?j=false).
-      { apply Nat.eqb_neq. omega. }
-      simpl in H1. rewrite H1. simpl. assert (j<=? S n=true).
-      { apply leb_correct. omega. }
-      rewrite H2. simpl.
-      f_equal. f_equal. assert (n>0) by (apply Nat.eqb_neq in ni; omega).
-      omega.
-    * apply leb_complete in iln. apply leb_complete_conv in jln. omega.
-  - apply leb_complete_conv in iln.
-    assert (1+i<=?n=false) by (apply leb_correct_conv; omega).
-    simpl in H. rewrite H. simpl. rewrite nj. simpl.
-    destruct (j<=?n) eqn:jln.
-    * simpl. assert (i<=?n-1=false).
-      { apply leb_correct_conv. omega. }
-      rewrite H0. reflexivity.
-    * simpl. assert (i<=?n=false) by (apply leb_correct_conv; omega).
-      rewrite H0. reflexivity.
+  - assert (1+i<=?i=false) by (apply leb_correct_conv; omega).
+    simpl in H. rewrite H. simpl.
+    assert (j<=?i=true) by (apply leb_correct;omega).
+    rewrite H0. rewrite eqij. simpl. rewrite H0.
+    assert (i<=?i-1=false).
+    { apply leb_correct_conv. apply Nat.eqb_neq in eqij. 
+      apply leb_complete in H0. omega. }
+    rewrite H1. reflexivity.
++ destruct (n=?j) eqn:nj.
+  ++apply Nat.eqb_eq in nj. subst.
+    assert (1+i<=?j=false) by (apply leb_correct_conv; omega).
+    simpl in H. rewrite H.
+    simpl. assert (j=?j=true) by (apply Nat.eqb_eq; omega).
+    rewrite H0. rewrite v_negshift_shift. rewrite v_negshift_shift. simpl.
+    rewrite v_shift_0. rewrite v_shift_0.
+    reflexivity. omega. omega.
+  ++destruct (i<=?n) eqn:iln; simpl.
+    - destruct (j<=?n) eqn:jln; simpl.
+      * apply leb_complete in jln. apply leb_complete in iln.
+        assert (i<=?n-1=true).
+        { apply leb_correct. apply Nat.eqb_neq in ni. omega. }
+        rewrite H. simpl. assert (1+i<=?n=true).
+        { apply leb_correct. apply leb_complete in H.
+          apply Nat.eqb_neq in ni. omega. }
+        simpl in H0. rewrite H0. simpl. 
+        assert (1+n=?j=false).
+        { apply Nat.eqb_neq. omega. }
+        simpl in H1. rewrite H1. simpl. assert (j<=? S n=true).
+        { apply leb_correct. omega. }
+        rewrite H2. simpl.
+        f_equal. f_equal. assert (n>0) by (apply Nat.eqb_neq in ni; omega).
+        omega.
+      * apply leb_complete in iln. apply leb_complete_conv in jln. omega.
+    - apply leb_complete_conv in iln.
+      assert (1+i<=?n=false) by (apply leb_correct_conv; omega).
+      simpl in H. rewrite H. simpl. rewrite nj. simpl.
+      destruct (j<=?n) eqn:jln.
+      * simpl. assert (i<=?n-1=false).
+        { apply leb_correct_conv. omega. }
+        rewrite H0. reflexivity.
+      * simpl. assert (i<=?n=false) by (apply leb_correct_conv; omega).
+        rewrite H0. reflexivity.
 }     
 all: f_equal; auto.
-+ clear v_shift_sub h_shift_sub.
-  unfold c_sub in c_shift_sub. rewrite v_shift_comm_aux. rewrite c_shift_sub.
-  f_equal. f_equal. f_equal. rewrite (v_shift_comm_aux 1 j). f_equal.
-  rewrite (v_shift_comm_aux 1 i). f_equal. all: omega.
-+ clear v_shift_sub h_shift_sub.
-  unfold c_sub in c_shift_sub. rewrite v_shift_comm_aux. rewrite c_shift_sub.
-  f_equal. f_equal. f_equal. rewrite (v_shift_comm_aux 1 j). f_equal.
-  rewrite (v_shift_comm_aux 1 i). f_equal. all: omega.
-+ apply h_shift_sub. auto.
+3: apply h_shift_sub; auto.
+all: clear v_shift_sub h_shift_sub; unfold c_sub in c_shift_sub.
+all: rewrite v_shift_comm_aux; try omega.
+all: rewrite c_shift_sub; clear c_shift_sub; try omega.
+all: do 3 f_equal; rewrite (v_shift_comm_aux 1 j); f_equal; try omega.
+all: rewrite (v_shift_comm_aux 1 i); f_equal; omega.
 }{
 induction c; unfold c_sub; simpl; f_equal;
 try apply v_shift_sub; try assumption.
-+ clear v_shift_sub h_shift_sub.
-  unfold c_sub in c_shift_sub. rewrite <-(v_shift_shift 1).
-  rewrite (v_shift_comm_aux 1 j). rewrite (v_shift_comm_aux 1 (1+j)). simpl.
-  rewrite c_shift_sub. clear c_shift_sub.
-  f_equal. f_equal. all: try omega.
-  rewrite <-(v_shift_shift 1 1 0). rewrite (v_shift_comm_aux 1 j).
-  rewrite (v_shift_comm_aux 1 (1+j)). f_equal. rewrite (v_shift_comm_aux 1 i).
-  rewrite (v_shift_comm_aux 1 (1+i)). f_equal. f_equal. all: omega.
-+ clear v_shift_sub h_shift_sub.
-  unfold c_sub in c_shift_sub. rewrite v_shift_comm_aux. rewrite c_shift_sub.
-  f_equal. f_equal. f_equal. rewrite (v_shift_comm_aux 1 j). f_equal.
+all: clear v_shift_sub h_shift_sub; unfold c_sub in c_shift_sub.
++ rewrite <-(v_shift_shift 1), (v_shift_comm_aux 1 j).
+  rewrite (v_shift_comm_aux 1 (1+j)), c_shift_sub. clear c_shift_sub. simpl.
+  do 2 f_equal. all: try omega.
+  rewrite <-(v_shift_shift 1 1 0), (v_shift_comm_aux 1 j).
+  rewrite (v_shift_comm_aux 1 (1+j)). f_equal. 
+  rewrite (v_shift_comm_aux 1 i), (v_shift_comm_aux 1 (1+i)). 
+  do 2 f_equal. all: omega.
++ rewrite v_shift_comm_aux. rewrite c_shift_sub. clear c_shift_sub.
+  do 3 f_equal. rewrite (v_shift_comm_aux 1 j). f_equal.
   rewrite (v_shift_comm_aux 1 i). f_equal. all: omega.
-+ clear v_shift_sub h_shift_sub.
-  unfold c_sub in c_shift_sub. rewrite v_shift_comm_aux. rewrite c_shift_sub.
-  f_equal. f_equal. f_equal. rewrite (v_shift_comm_aux 1 j). f_equal.
++ rewrite v_shift_comm_aux. rewrite c_shift_sub. clear c_shift_sub.
+  do 3 f_equal. rewrite (v_shift_comm_aux 1 j). f_equal.
   rewrite (v_shift_comm_aux 1 i). f_equal. all: omega.
-+ clear v_shift_sub h_shift_sub.
-  unfold c_sub in c_shift_sub. rewrite v_shift_comm_aux. rewrite c_shift_sub.
-  f_equal. f_equal. f_equal. rewrite (v_shift_comm_aux 1 j). f_equal.
++ rewrite v_shift_comm_aux. rewrite c_shift_sub. clear c_shift_sub.
+  do 3 f_equal. rewrite (v_shift_comm_aux 1 j). f_equal.
   rewrite (v_shift_comm_aux 1 i). f_equal. all: omega.
-+ clear v_shift_sub h_shift_sub.
-  unfold c_sub in c_shift_sub. rewrite <-(v_shift_shift 1).
-  rewrite (v_shift_comm_aux 1 j). rewrite (v_shift_comm_aux 1 (1+j)). simpl.
-  rewrite c_shift_sub. clear c_shift_sub.
-  f_equal. f_equal. all: try omega.
-  rewrite <-(v_shift_shift 1 1 0). rewrite (v_shift_comm_aux 1 j).
-  rewrite (v_shift_comm_aux 1 (1+j)). f_equal. rewrite (v_shift_comm_aux 1 i).
-  rewrite (v_shift_comm_aux 1 (1+i)). f_equal. f_equal. all: omega.
-+ clear v_shift_sub h_shift_sub.
-  unfold c_sub in c_shift_sub. rewrite v_shift_comm_aux. rewrite c_shift_sub.
-  f_equal. f_equal. f_equal. rewrite (v_shift_comm_aux 1 j). f_equal.
++ rewrite <-(v_shift_shift 1), (v_shift_comm_aux 1 j).
+  rewrite (v_shift_comm_aux 1 (1+j)), c_shift_sub. clear c_shift_sub. simpl.
+  do 2 f_equal. all: try omega.
+  rewrite <-(v_shift_shift 1 1 0), (v_shift_comm_aux 1 j).
+  rewrite (v_shift_comm_aux 1 (1+j)). f_equal. 
+  rewrite (v_shift_comm_aux 1 i), (v_shift_comm_aux 1 (1+i)). 
+  do 2 f_equal. all: omega.
++ rewrite v_shift_comm_aux. rewrite c_shift_sub. clear c_shift_sub.
+  do 3 f_equal. rewrite (v_shift_comm_aux 1 j). f_equal.
   rewrite (v_shift_comm_aux 1 i). f_equal. all: omega.
-+ clear v_shift_sub h_shift_sub.
-  unfold c_sub in c_shift_sub. rewrite v_shift_comm_aux. rewrite c_shift_sub.
-  f_equal. f_equal. f_equal. rewrite (v_shift_comm_aux 1 j). f_equal.
++ rewrite v_shift_comm_aux. rewrite c_shift_sub. clear c_shift_sub.
+  do 3 f_equal. rewrite (v_shift_comm_aux 1 j). f_equal.
   rewrite (v_shift_comm_aux 1 i). f_equal. all: omega.
 }{
 induction h; unfold h_sub; simpl. auto. f_equal.
 + apply h_shift_sub. assumption.
 + clear v_shift_sub h_shift_sub.
-  unfold c_sub in c_shift_sub. rewrite <-(v_shift_shift 1).
-  rewrite (v_shift_comm_aux 1 j). rewrite (v_shift_comm_aux 1 (1+j)). simpl.
-  rewrite c_shift_sub. clear c_shift_sub.
-  f_equal. f_equal. all: try omega.
-  rewrite <-(v_shift_shift 1 1 0). rewrite (v_shift_comm_aux 1 j).
-  rewrite (v_shift_comm_aux 1 (1+j)). f_equal. rewrite (v_shift_comm_aux 1 i).
-  rewrite (v_shift_comm_aux 1 (1+i)). f_equal. f_equal. all: omega.
+  unfold c_sub in c_shift_sub.
+  rewrite <-(v_shift_shift 1), (v_shift_comm_aux 1 j).
+  rewrite (v_shift_comm_aux 1 (1+j)), c_shift_sub. clear c_shift_sub. simpl.
+  do 2 f_equal. all: try omega.
+  rewrite <-(v_shift_shift 1 1 0), (v_shift_comm_aux 1 j).
+  rewrite (v_shift_comm_aux 1 (1+j)). f_equal. 
+  rewrite (v_shift_comm_aux 1 i), (v_shift_comm_aux 1 (1+i)). 
+  do 2 f_equal. all: omega.
 }
 Qed.
+
+
+Lemma v_negshift_sub v v' i j (safe: j <= i): 
+  v_no_var v i -> v_no_var v' i ->
+  Sub.v_negshift (v_sub v v' j) 1 i = 
+  (v_sub (Sub.v_negshift v 1 (i+1)) (Sub.v_negshift v' 1 i) j)
+with c_negshift_sub c v' i j (safe: j <= i): 
+  c_no_var c i -> v_no_var v' i ->
+  Sub.c_negshift (c_sub c v' j) 1 i = 
+  (c_sub (Sub.c_negshift c 1 (i+1)) (Sub.v_negshift v' 1 i) j)
+with h_negshift_sub h v' i j (safe: j <= i): 
+  h_no_var h i -> v_no_var v' i ->
+  Sub.h_negshift (h_sub h v' j) 1 i = 
+  (h_sub (Sub.h_negshift h 1 (i+1)) (Sub.v_negshift v' 1 i) j).
+Proof.
+{
+intros nov nov'. destruct v; unfold v_sub; simpl.
+{
+clear v_negshift_sub c_negshift_sub h_negshift_sub.
+destruct v as (x, n). 
+destruct (n=?j) eqn:nj.
+apply Nat.eqb_eq in nj. subst.
+
+(* HERE WE ARE *)
+
+
++ destruct (i+1=?j) eqn:eqij.
+  - apply Nat.eqb_eq in eqij. subst.
+    assert (1+j<=?j=false) by (apply leb_correct_conv; omega).
+    simpl in H. rewrite H. simpl.
+    assert (j=?j=true) by (apply Nat.eqb_eq; reflexivity).
+    rewrite H0. simpl. 
+    rewrite v_negshift_shift. rewrite v_negshift_shift.
+    rewrite v_shift_shift. rewrite v_shift_shift. f_equal.
+    omega. omega.
+  - assert (1+i<=?i=false) by (apply leb_correct_conv; omega).
+    simpl in H. rewrite H. simpl.
+    assert (j<=?i=true) by (apply leb_correct;omega).
+    rewrite H0. rewrite eqij. simpl. rewrite H0.
+    assert (i<=?i-1=false).
+    { apply leb_correct_conv. apply Nat.eqb_neq in eqij. 
+      apply leb_complete in H0. omega. }
+    rewrite H1. reflexivity.
++ destruct (n=?j) eqn:nj.
+  ++apply Nat.eqb_eq in nj. subst.
+    assert (1+i<=?j=false) by (apply leb_correct_conv; omega).
+    simpl in H. rewrite H.
+    simpl. assert (j=?j=true) by (apply Nat.eqb_eq; omega).
+    rewrite H0. rewrite v_negshift_shift. rewrite v_negshift_shift. simpl.
+    rewrite v_shift_0. rewrite v_shift_0.
+    reflexivity. omega. omega.
+  ++destruct (i<=?n) eqn:iln; simpl.
+    - destruct (j<=?n) eqn:jln; simpl.
+      * apply leb_complete in jln. apply leb_complete in iln.
+        assert (i<=?n-1=true).
+        { apply leb_correct. apply Nat.eqb_neq in ni. omega. }
+        rewrite H. simpl. assert (1+i<=?n=true).
+        { apply leb_correct. apply leb_complete in H.
+          apply Nat.eqb_neq in ni. omega. }
+        simpl in H0. rewrite H0. simpl. 
+        assert (1+n=?j=false).
+        { apply Nat.eqb_neq. omega. }
+        simpl in H1. rewrite H1. simpl. assert (j<=? S n=true).
+        { apply leb_correct. omega. }
+        rewrite H2. simpl.
+        f_equal. f_equal. assert (n>0) by (apply Nat.eqb_neq in ni; omega).
+        omega.
+      * apply leb_complete in iln. apply leb_complete_conv in jln. omega.
+    - apply leb_complete_conv in iln.
+      assert (1+i<=?n=false) by (apply leb_correct_conv; omega).
+      simpl in H. rewrite H. simpl. rewrite nj. simpl.
+      destruct (j<=?n) eqn:jln.
+      * simpl. assert (i<=?n-1=false).
+        { apply leb_correct_conv. omega. }
+        rewrite H0. reflexivity.
+      * simpl. assert (i<=?n=false) by (apply leb_correct_conv; omega).
+        rewrite H0. reflexivity.
+}     
+all: f_equal; auto.
+3: apply h_shift_sub; auto.
+all: clear v_shift_sub h_shift_sub; unfold c_sub in c_shift_sub.
+all: rewrite v_shift_comm_aux; try omega.
+all: rewrite c_shift_sub; clear c_shift_sub; try omega.
+all: do 3 f_equal; rewrite (v_shift_comm_aux 1 j); f_equal; try omega.
+all: rewrite (v_shift_comm_aux 1 i); f_equal; omega.
+}{
+induction c; unfold c_sub; simpl; f_equal;
+try apply v_shift_sub; try assumption.
+all: clear v_shift_sub h_shift_sub; unfold c_sub in c_shift_sub.
++ rewrite <-(v_shift_shift 1), (v_shift_comm_aux 1 j).
+  rewrite (v_shift_comm_aux 1 (1+j)), c_shift_sub. clear c_shift_sub. simpl.
+  do 2 f_equal. all: try omega.
+  rewrite <-(v_shift_shift 1 1 0), (v_shift_comm_aux 1 j).
+  rewrite (v_shift_comm_aux 1 (1+j)). f_equal. 
+  rewrite (v_shift_comm_aux 1 i), (v_shift_comm_aux 1 (1+i)). 
+  do 2 f_equal. all: omega.
++ rewrite v_shift_comm_aux. rewrite c_shift_sub. clear c_shift_sub.
+  do 3 f_equal. rewrite (v_shift_comm_aux 1 j). f_equal.
+  rewrite (v_shift_comm_aux 1 i). f_equal. all: omega.
++ rewrite v_shift_comm_aux. rewrite c_shift_sub. clear c_shift_sub.
+  do 3 f_equal. rewrite (v_shift_comm_aux 1 j). f_equal.
+  rewrite (v_shift_comm_aux 1 i). f_equal. all: omega.
++ rewrite v_shift_comm_aux. rewrite c_shift_sub. clear c_shift_sub.
+  do 3 f_equal. rewrite (v_shift_comm_aux 1 j). f_equal.
+  rewrite (v_shift_comm_aux 1 i). f_equal. all: omega.
++ rewrite <-(v_shift_shift 1), (v_shift_comm_aux 1 j).
+  rewrite (v_shift_comm_aux 1 (1+j)), c_shift_sub. clear c_shift_sub. simpl.
+  do 2 f_equal. all: try omega.
+  rewrite <-(v_shift_shift 1 1 0), (v_shift_comm_aux 1 j).
+  rewrite (v_shift_comm_aux 1 (1+j)). f_equal. 
+  rewrite (v_shift_comm_aux 1 i), (v_shift_comm_aux 1 (1+i)). 
+  do 2 f_equal. all: omega.
++ rewrite v_shift_comm_aux. rewrite c_shift_sub. clear c_shift_sub.
+  do 3 f_equal. rewrite (v_shift_comm_aux 1 j). f_equal.
+  rewrite (v_shift_comm_aux 1 i). f_equal. all: omega.
++ rewrite v_shift_comm_aux. rewrite c_shift_sub. clear c_shift_sub.
+  do 3 f_equal. rewrite (v_shift_comm_aux 1 j). f_equal.
+  rewrite (v_shift_comm_aux 1 i). f_equal. all: omega.
+}{
+induction h; unfold h_sub; simpl. auto. f_equal.
++ apply h_shift_sub. assumption.
++ clear v_shift_sub h_shift_sub.
+  unfold c_sub in c_shift_sub.
+  rewrite <-(v_shift_shift 1), (v_shift_comm_aux 1 j).
+  rewrite (v_shift_comm_aux 1 (1+j)), c_shift_sub. clear c_shift_sub. simpl.
+  do 2 f_equal. all: try omega.
+  rewrite <-(v_shift_shift 1 1 0), (v_shift_comm_aux 1 j).
+  rewrite (v_shift_comm_aux 1 (1+j)). f_equal. 
+  rewrite (v_shift_comm_aux 1 i), (v_shift_comm_aux 1 (1+i)). 
+  do 2 f_equal. all: omega.
+}
+Qed.
+
 
 Fixpoint v_under_var_shift v j n cut:
   v_under_var v j -> cut <= j -> v_under_var (Sub.v_shift v n cut) (n+j)
@@ -480,6 +623,29 @@ with c_shift_too_high c n cut :
   c_under_var c cut -> Sub.c_shift c n cut = c
 with h_shift_too_high h n cut :
   h_under_var h cut -> Sub.h_shift h n cut = h.
+Proof.
+{
+intros under. destruct v; simpl; simpl in under.
+{ destruct v.
+  assert (cut <=? v0 = false) by (apply leb_correct_conv; omega).
+  rewrite H. reflexivity. }
+all: try (destruct under; f_equal; auto) || (f_equal; auto).
+}{
+intros under. destruct c; simpl; simpl in under.
+all: try (destruct under; f_equal; auto) || (f_equal; auto).
+all: destruct H0; auto.
+}{
+intros under. destruct h; simpl; simpl in under.
+all: try (destruct under; f_equal; auto) || (f_equal; auto).
+}
+Qed.
+
+Fixpoint v_negshift_too_high v n cut :
+  v_under_var v cut -> Sub.v_negshift v n cut = v
+with c_negshift_too_high c n cut :
+  c_under_var c cut -> Sub.c_negshift c n cut = c
+with h_negshift_too_high h n cut :
+  h_under_var h cut -> Sub.h_negshift h n cut = h.
 Proof.
 {
 intros under. destruct v; simpl; simpl in under.
